Added RecordedViewChangeMsgsCameFromNetwork predicate to the global Invariant.
We need to retain the information that the recorded ViewChangeMsgs in the replicas
came from the network.
Minor fixes and structuring of the code by adding the necessary proofs for the
newly added predicates in the global Invariant - HonestReplicasLeaveViewsBehind,
RecordedNewViewMsgsContainSentVCMsgs and RecordedViewChangeMsgsCameFromNetwork.

docs/sbft-formal-model/proof.dfy
@@ -311,6 +311,7 @@ module Proof {
     && UnCommitableAgreesWithRecordedPrePrepare(c, v)
     && HonestReplicasLeaveViewsBehind(c, v)
     && RecordedNewViewMsgsContainSentVCMsgs(c, v)
+    && RecordedViewChangeMsgsCameFromNetwork(c, v)
   }
 
   function sentPreparesForSeqID(c: Constants, v:Variables, view:nat, seqID:Messages.SequenceID,
@@ -1041,13 +1042,16 @@ module Proof {
   }
 
   predicate {:opaque} HonestReplicasLeaveViewsBehind(c:Constants, v:Variables) {
+    && v.WF(c)
     && (forall viewChangeMsg | && viewChangeMsg in v.network.sentMsgs
+                               && viewChangeMsg.payload.ViewChangeMsg?
                                && IsHonestReplica(c, viewChangeMsg.sender)
                                   :: && var replicaVariables := v.hosts[viewChangeMsg.sender].replicaVariables;
                                      && replicaVariables.view >= viewChangeMsg.payload.newView)
   }
 
   predicate {:opaque} RecordedNewViewMsgsContainSentVCMsgs(c:Constants, v:Variables) {
+    && v.WF(c)
     && (forall replicaIdx, newViewMsg | && IsHonestReplica(c, replicaIdx)
                                         && var replicaVariables := v.hosts[replicaIdx].replicaVariables;
                                         && newViewMsg in replicaVariables.newViewMsgsRecvd.msgs
@@ -1066,6 +1070,14 @@ module Proof {
                    && replicaVars.view == replicaVars.workingWindow.prePreparesRcvd[seqID].value.payload.view)
   }
 
+  predicate {:opaque} RecordedViewChangeMsgsCameFromNetwork(c:Constants, v:Variables) {
+    && v.WF(c)
+    && (forall replicaIdx, viewChangeMsg | 
+                              && IsHonestReplica(c, replicaIdx)
+                              && var replicaVariables := v.hosts[replicaIdx].replicaVariables;
+                              && viewChangeMsg in replicaVariables.viewChangeMsgsRecvd.msgs
+                                 :: viewChangeMsg in v.network.sentMsgs)
+  }
 
 //TODO: write a predicate Prepare matches Commit
   lemma GetPrepareFromHonestSenderForCommit(c:Constants, v:Variables, commitMsg:Message)
@@ -1276,6 +1288,71 @@ module Proof {
     }
   }
 
+  lemma HonestPreservesHonestReplicasLeaveViewsBehind(c: Constants, v:Variables, v':Variables, step:Step, h_v:Replica.Variables, h_step:Replica.Step)
+    requires Inv(c, v)
+    requires HonestReplicaStepTaken(c, v, v', step, h_v, h_step)
+    ensures HonestReplicasLeaveViewsBehind(c, v')
+  {
+    reveal_HonestReplicasLeaveViewsBehind();
+  }
+
+  lemma HonestPreservesRecordedNewViewMsgsContainSentVCMsgs(c: Constants, v:Variables, v':Variables, step:Step, h_v:Replica.Variables, h_step:Replica.Step)
+    requires Inv(c, v)
+    requires HonestReplicaStepTaken(c, v, v', step, h_v, h_step)
+    ensures RecordedNewViewMsgsContainSentVCMsgs(c, v')
+  {
+    if(h_step.SelectQuorumOfViewChangeMsgsStep?) {
+      reveal_RecordedNewViewMsgsContainSentVCMsgs();
+      reveal_RecordedViewChangeMsgsCameFromNetwork();
+      forall replicaIdx, newViewMsg | && IsHonestReplica(c, replicaIdx)
+                                        && var replicaVariables := v'.hosts[replicaIdx].replicaVariables;
+                                        && newViewMsg in replicaVariables.newViewMsgsRecvd.msgs
+                                           ensures newViewMsg.payload.vcMsgs.msgs <= v'.network.sentMsgs {
+
+        if newViewMsg in v.hosts[replicaIdx].replicaVariables.newViewMsgsRecvd.msgs {
+          assert newViewMsg.payload.vcMsgs.msgs <= v'.network.sentMsgs;
+        } else {
+          assert newViewMsg.payload.vcMsgs.msgs <= step.msgOps.signedMsgsToCheck;
+          assert step.msgOps.signedMsgsToCheck <= v.network.sentMsgs;
+          assert newViewMsg.payload.vcMsgs.msgs <= v'.network.sentMsgs;
+        }
+      }
+
+      assert RecordedNewViewMsgsContainSentVCMsgs(c, v');
+    } else if(h_step.RecvNewViewMsgStep?) {
+      reveal_RecordedNewViewMsgsContainSentVCMsgs();
+      assert RecordedNewViewMsgsContainSentVCMsgs(c, v');
+    } else {
+      reveal_RecordedNewViewMsgsContainSentVCMsgs();
+      assert RecordedNewViewMsgsContainSentVCMsgs(c, v');
+    }
+
+    
+  }
+
+  lemma HonestPreservesRecordedViewChangeMsgsCameFromNetwork(c: Constants, v:Variables, v':Variables, step:Step, h_v:Replica.Variables, h_step:Replica.Step)
+    requires Inv(c, v)
+    requires HonestReplicaStepTaken(c, v, v', step, h_v, h_step)
+    ensures RecordedViewChangeMsgsCameFromNetwork(c, v')
+  {
+    reveal_RecordedViewChangeMsgsCameFromNetwork();
+    forall replicaIdx, viewChangeMsg | 
+                              && IsHonestReplica(c, replicaIdx)
+                              && var replicaVariables := v'.hosts[replicaIdx].replicaVariables;
+                              && viewChangeMsg in replicaVariables.viewChangeMsgsRecvd.msgs
+                                 ensures viewChangeMsg in v'.network.sentMsgs {
+      if viewChangeMsg !in v.network.sentMsgs {
+        if(h_step.RecvViewChangeMsgStep?) {
+          assert viewChangeMsg in v'.network.sentMsgs;
+        } else if(h_step.LeaveViewStep?){
+          assert viewChangeMsg in v'.network.sentMsgs;
+        } else {
+          assert false;
+        }
+      }
+    }
+  }
+
   lemma HonestRecvPrePrepareStepPreservesUnCommitableAgreesWithRecordedPrePrepare(c: Constants, v:Variables, v':Variables, step:Step, h_v:Replica.Variables, h_step:Replica.Step)
     requires Inv(c, v)
     requires HonestReplicaStepTaken(c, v, v', step, h_v, h_step)
@@ -1357,6 +1434,8 @@ module Proof {
       HonestLeaveViewStepPreservesUnCommitableAgreesWithRecordedPrePrepare(c, v, v', step, h_v, h_step);
     } else if(h_step.RecvPrePrepareStep?) {
       HonestRecvPrePrepareStepPreservesUnCommitableAgreesWithRecordedPrePrepare(c, v, v', step, h_v, h_step);
+    } else if(h_step.SendPrePrepareStep?) {
+      assume false;
     } else {
       TriviallyPreserveUnCommitableAgreesWithRecordedPrePrepare(c, v, v', step, HonestInfo(h_v, h_step));
     }
@@ -1393,6 +1472,9 @@ module Proof {
       HonestPreservesRecordedPrePreparesMatchHostView(c, v, v', step, h_v, h_step);
       HonestPreservesUnCommitableAgreesWithRecordedPrePrepare(c, v, v', step, h_v, h_step);
       HonestPreservesUnCommitableAgreesWithPrepare(c, v, v', step, h_v, h_step);
+      HonestPreservesHonestReplicasLeaveViewsBehind(c, v, v', step, h_v, h_step);
+      HonestPreservesRecordedNewViewMsgsContainSentVCMsgs(c, v, v', step, h_v, h_step);
+      HonestPreservesRecordedViewChangeMsgsCameFromNetwork(c, v, v', step, h_v, h_step);
     } else {
       InvNextFaultyOrClient(c, v, v', step);
     }
@@ -1465,7 +1547,15 @@ module Proof {
     assert UnCommitableAgreesWithPrepare(c, v') by {
       TriviallyPreserveUnCommitableAgreesWithPrepare(c, v, v', step, NotHonest());
     }
-    
+    assert HonestReplicasLeaveViewsBehind(c, v') by {
+      reveal_HonestReplicasLeaveViewsBehind();
+    }
+    assert RecordedNewViewMsgsContainSentVCMsgs(c, v') by {
+      reveal_RecordedNewViewMsgsContainSentVCMsgs();
+    }
+    assert RecordedViewChangeMsgsCameFromNetwork(c, v') by {
+      reveal_RecordedViewChangeMsgsCameFromNetwork();
+    }
   }
 
   lemma InitEstablishesInv(c: Constants, v:Variables)
@@ -1492,6 +1582,9 @@ module Proof {
       reveal_RecordedPrePreparesMatchHostView();
       reveal_UnCommitableAgreesWithPrepare();
       reveal_UnCommitableAgreesWithRecordedPrePrepare();
+      reveal_HonestReplicasLeaveViewsBehind();
+      reveal_RecordedNewViewMsgsContainSentVCMsgs();
+      reveal_RecordedViewChangeMsgsCameFromNetwork();
     }
   }
 
